\documentclass{ximera}
\title{Review of week 2}

\begin{document}
	\begin{abstract}
		Test yo skillz on these sweet practice problems
	\end{abstract}
	
	This section just contains practice problems on the material we have learned this week.  These problems do not have detailed hints:  \textbf{clicking on the hint will
	immediately reveal the answer}.  Use them to test your knowledge.  If you are confused about how to do any of these problems, ask your peers in one of the forums.
	\\
	\\
	\textbf{Computing the Jacobian}
	\\
	\\
	\begin{question}	
		Compute the Jacobian of $f:\R^2 \to \R^3$ defined by $f(x,y) = (\sin(xy),x^2y^3, x^3)$.
		\begin{solution}
		\begin{hint}
			\(J = \begin{bmatrix} y\cos(xy) & x\cos(xy) \\ 2xy^4 & 3x^2y^2 \\ 3x^2 & 0 \end{bmatrix}\)
		\end{hint}
		\begin{matrix-answer}[name=J]
			correct-Matrix  = [['y(cos(xy))','x(cos(xy))'],['2xy^4','3x^2y^2'],['3x^2','0']]
		\end{matrix-answer}
		\end{solution}
	\end{question}
	
	\begin{question}	
		Compute the Jacobian of $f:\R^4 - \{y=0\} \to \R^1$ defined by $f(x,y,z,t) = x^2yz^3t^4+\frac{x}{y}$.
		\begin{solution}
		\begin{hint}
			\(J = \begin{bmatrix} 2xyz^3t^4 +\frac{1}{y} & x^2z^3t^4 - \frac{x}{y^2} & 3x^2yz^2t^4 & 4x^2yz^3t^3\end{bmatrix}\)
		\end{hint}
		\begin{matrix-answer}[name=J]
			correct-Matrix  = [['2xyz^3t^4 +1/y','x^2z^3t^4 - xy^(-2)', '3x^2yz^2t^4', '4x^2yz^3t^3']]
		\end{matrix-answer}
		\end{solution}
	\end{question}
	
	\begin{question}	
		Compute the Jacobian of $f:\R^2 - \{(0,0)\} \to \R^2$ defined by $f(x,y) = (\frac{x}{x^2+y^2},\frac{y}{x^2+y^2})$.
		\begin{solution}
		\begin{hint}
			\(J = \begin{bmatrix} \frac{y^2-x^2}{(x^2+y^2)^2} & \frac{-2xy}{(x^2+y^2)^2} \\   \frac{-2xy}{(x^2+y^2)^2} & \frac{x^2-y^2}{(x^2+y^2)^2}  \end{bmatrix}\)
		\end{hint}
		\begin{matrix-answer}[name=J]
			correct-Matrix  = [['(y^2-x^2)/(x^2+y^2)^2', ' -2xy/(x^2+y^2)^2'],['-2xy/(x^2+y^2)^2','(x^2-y^2)/(x^2+y^2)^2']]
		\end{matrix-answer}
		\end{solution}
	\end{question}
	
	\begin{question}	
		Compute the Jacobian of $f:\R \to \R^4$ defined by $f(t) = (\cos(t),\sin(t),t,t^2)$.
		\begin{solution}
		\begin{hint}
			\(J = \verticalvector{-\sin(r)\\ \cos(t) \\ 1 \\ 2t}\)
		\end{hint}
		\begin{matrix-answer}[name=J]
			correct-Matrix  = [['-sin(t)'],['cos(t)'],['1'],['2t']]
		\end{matrix-answer}
		\end{solution}
	\end{question}
	\\
	\\
	\textbf{Computing the Gradient Vector}	
	\\
	\\
	\begin{question}	
		Compute the $\nabla f$ where $f:\R^3 \to \R$ defined by $f(x,y,z) = x^2+xyz$.
		\begin{solution}
		\begin{hint}
			\(J = \verticalvector{2x+yz\\ xz \\xy}\)
		\end{hint}
		\begin{matrix-answer}[name=J]
			correct-Matrix  = [['2x+yz'],['xz'],['xy']]
		\end{matrix-answer}
		\end{solution}
	\end{question}
	
	\begin{question}	
		Compute the $\nabla f$ where $f:\R^4 \to \R$ defined by $f(x,y,z,t) = \cos(xy)\sin(zt)$.
		\begin{solution}
		\begin{hint}
			\(J = \verticalvector{-y\sin(xy)\sin(zt)\\ -x\sin(xy)\sin(zt) \\ t\cos(xy)\cos(zt) \\ z\cos(xy)\cos(zt)}\)
		\end{hint}
		\begin{matrix-answer}[name=J]
			correct-Matrix  = [['-x(sin(xy)sin(zt))'],['-y(sin(xy)sin(zt))'],['t(cos(xy)cos(zt))'],['z(cos(xy)cos(zt))']]
		\end{matrix-answer}
		\end{solution}
	\end{question}
	
	\begin{question}	
		Compute the $\nabla f$ where $f:\R^2-{(0,0)} \to \R$ defined by $f(x,y) = \frac{x}{y}$.
		\begin{solution}
		\begin{hint}
			\(J = \verticalvector{\frac{1}{y} \\ \frac{-x}{y^2}}\)
		\end{hint}
		\begin{matrix-answer}[name=J]
			correct-Matrix  = [['1/y'],['-x/y^2']]
		\end{matrix-answer}
		\end{solution}
	\end{question}
	\\
	\\
	\textbf{Linear Approximation}
	\\
	\\
	\begin{question}
		Let $f:\R^2 \to \R^2$ be given by $f(x,y) = (x^2-y^2,2xy)$.
		\begin{solution}
			\begin{hint}
				$\verticalvector{8.02\\7.4}$
			\end{hint}
			Use the linear approximation to $f$ at $(3,1)$ to approximate $f(3.1,2.3)$.  Give your answer as a column vector.
			\begin{matrix-answer}
				correctMatrix = [['8.02'],[7.4]]
			\end{matrix-answer}
		\end{solution}
	\end{question}
	
	\begin{question}
		Let $f:\R^1 \to \R^3$ be given by $f(t) = (t,t^2,t^3)$.
		\begin{solution}
			\begin{hint}
				$\verticalvector{1.1\\1.2\\1.3}$
			\end{hint}
			Use the linear approximation to $f$ at $1$ to approximate $f(1.1)$.  Give your answer as a column vector.
			\begin{matrix-answer}
				correctMatrix = [['1.1'],['1.2'],['1.3']]
			\end{matrix-answer}
		\end{solution}
	\end{question}
	
    \begin{question}
		Let $f:\R^3\to \R^2$ be given by $f(x,y,z) = (xy,yz)$.
		\begin{solution}
			\begin{hint}
				$\verticalvector{2.1\\6.1}$
			\end{hint}

			Use the linear approximation to $f$ at $(1,2,3)$ to approximate $f(1.1,1.9,3.2)$.  Give your answer as a column vector.
			\begin{matrix-answer}
				correctMatrix = [['2.1'],['6.1']]
			\end{matrix-answer}
		\end{solution}
	\end{question}	
	\\
	\\
	\textbf{Increasing or Decreasing?}
	\\
	\\
	\begin{question}
		Let $f:\R^2 \to \R$ be given by $f(x,y)=(x+2y)^2+y^3$
		\begin{solution}
			\begin{hint}
				By computing the directional derivative in that direction, we see that $f$ is decreasing. 
			\end{hint}
			At the point $(-1,5)$, is $f$ increasing or decreasing in the direction $\verticalvector{1\\-1}$.
			\begin{multiple-choice}
				\choice{Increasing}
				\choice[correct]{Decreasing}
			\end{multiple-choice}
		\end{solution}
	\end{question}
	
	\begin{question}
		Let $f:\R^3 \to \R$ be given by $f(x,y,z)=\frac{x+y}{z}$
		\begin{solution}
			\begin{hint}
				By computing the directional derivative in that direction, we see that $f$ is decreasing. 
				You could also see that $f$ is decreasing by noting that the numerator is left unchanged when $x$ and $y$ are increased
				equally in opposite directions, but the denominator is increasing.
			\end{hint}
			At the point $(3,2,6)$, is $f$ increasing or decreasing in the direction $\verticalvector{1\\-1\\2}$.
			\begin{multiple-choice}
				\choice{Increasing}
				\choice[correct]{Decreasing}
			\end{multiple-choice}
		\end{solution}
	\end{question}
	
	\begin{question}
		Let $f:\R^4 \to \R$ be given by $f(x,y,z,t)=\frac{xy^2}{t}+z^2$
		\begin{solution}
			\begin{hint}
				By computing the directional derivative in that direction, we see that $f$ is increasing.
			\end{hint}
			At the point $(0,1,5,-1)$, is $f$ increasing or decreasing in the direction $\verticalvector{1\\1\\-2\\3}$.
			\begin{multiple-choice}
				\choice[correct]{Increasing}
				\choice{Decreasing}
			\end{multiple-choice}
		\end{solution}
	\end{question}
	\\
	\\
	\textbf{Finding stationary points}
	\\
	\\
	\begin{question}
		Let $f:\R^2 \to \R^2$ be defined by $f(x,y) = (x^2-x-y^2,2xy-y) $.
		There are is one stationary point of $f$ (one place where the derivative vanishes).  
		What is this stationary point?  Give your answer as a column vector
		 
		 \begin{matrix-answer}
		 correctMatrix = [['1/2'],['0']]
		 \end{matrix-answer}
	\end{question}
	\\
	\\
	\begin{question}
		Let $f:\R^3 \to \R$ be defined by $f(x,y,z) = x^2+xy+xz+z^2 $.
		There are is one stationary point of $f$ (one place where the derivative vanishes).  
		What is this stationary point?  Give your answer as a column vector
		 
		 \begin{matrix-answer}
		 correctMatrix = [['0'],['0'],['0']]
		 \end{matrix-answer}
	\end{question}
	\\
	\\
	\begin{question}
		Let $f:\R^2 \to \R^3$ be given by $f(x,y) = (x^2,y-x,\sqrt{x^2-4x+4+y^2})$
		\begin{question}
			$f$ is differentiable everywhere except for one point.  What is that point?  Give your answer as a column vector
			\begin{matrix-answer}
			correctMatrix = [['2'],['0']]
			\end{matrix-answer}
		\end{question}
	\end{question}
	\\
	\\
	\textbf{Finding tangent hypersurfaces}
	\\
	\\
	\begin{question}
		\begin{hint}
			$4(x-2)-6(y-3) = 0$
		\end{hint}
		Let $f:\R^2 \to \R$ be defined by $f(x,y)=x^2-y^2$.
		\begin{question}
			The equation of the tangent line to the curve $f(x,y)=5$ at the point $(3,2)$ 
			is $0=$ \answer{$4(x-2)-6(y-3)$}
		\end{question}
	\end{question}
	
	\begin{question}
		\begin{hint}
			$4(x-3)-2y-2(z-1) = 0$
		\end{hint}
		Let $f:\R^3 \to \R$ be defined by $f(x,y)=$.
		\begin{question}
			The equation of the tangent plane to the surface $f(x,y,z)=3$ at the point $(3,0,1)$ 
			is $0=$ \answer{$4(x-3)-2y-2(z-1)$}
		\end{question}
	\end{question}
	\\
	\\
	\textbf{Using the Chain Rule}
			
	\begin{question}
		Let $f:\R^2 \to \R^2$ be defined by $f(x,y)=(x^2y+x,\frac{x}{y})$.  Let 
		$g:\R^2 \to \R^3$ be defined by $g(x,y) = (x+y,x-y,xy)$.  
		\begin{solution}
			\begin{hint}
				\(\begin{bmatrix} 
				2ab+1+\frac{1}{b}& a^2-\frac{a}{b^2}\\
				2ab+1-\frac{1}{b}& a^2+\frac{a}{b^2}\\
				3a^2+\frac{2a}{b} & \frac{-a^2}{b^2}
				\end{bmatrix}\)
			\end{hint}
		Use the chain rule to find the
		Jacobian of $(g \circ f)$ at the point $(a,b)$.
		
		\begin{matrix-answer}
			correctMatrix = [['2ab+1+1/b','a^2-a/b^2'],['2ab+1-1/b','a^2+a/b^2'],['3a^2+2a/b','-a^2/b^2']]
		\end{matrix-answer}
		\end{solution}
	\end{question}	
	
	\begin{question}
		Let $f:\R^2 \to \R$ be defined by $f(x,y)=x^3+y^3$.  Let 
		$g:\R \to \R^2$ be defined by $g(x,y) = (x, \sin(x))$.  
		\begin{solution}
			\begin{hint}
				\(\begin{bmatrix} 
				3a^2& 3b^2\\
				3a^2\cos(a^3+b^3)& 3b^2\cos(a^3+b^3)
				\end{bmatrix}\)
			\end{hint}
		Use the chain rule to find the
		Jacobian of $(g \circ f)$ at the point $(a,b)$.
		
		\begin{matrix-answer}
			correctMatrix = [['3a^2','3b^2'],['3a^2cos(a^3+b^3)','3b^2cos(a^3+b^3)']]
		\end{matrix-answer}
		\end{solution}
	\end{question}	
	
\end{document}