\documentclass{ximera}
\title{Use the chain rule}

\begin{document}
	\begin{abstract}
		Compute using the chain rule.
	\end{abstract}\maketitle
	
			
	\begin{question}
		Let $f:\R^2 \to \R^2$ be defined by $f(x,y)=(x^2y+x,\frac{x}{y})$.  Let 
		$g:\R^2 \to \R^3$ be defined by $g(x,y) = (x+y,x-y,xy)$.  
		\begin{solution}
			\begin{hint}
				\(\begin{bmatrix} 
				2ab+1+\frac{1}{b}& a^2-\frac{a}{b^2}\\
				2ab+1-\frac{1}{b}& a^2+\frac{a}{b^2}\\
				3a^2+\frac{2a}{b} & \frac{-a^2}{b^2}
				\end{bmatrix}\)
			\end{hint}
		Use the chain rule to find the
		Jacobian of $(g \circ f)$ at the point $(a,b)$.
		
		\begin{matrix-answer}
			correctMatrix = [['2ab+1+1/b','a^2-a/b^2'],['2ab+1-1/b','a^2+a/b^2'],['3a^2+2a/b','-a^2/b^2']]
		\end{matrix-answer}
		\end{solution}
	\end{question}	
	
	\begin{question}
		Let $f:\R^2 \to \R$ be defined by $f(x,y)=x^3+y^3$.  Let 
		$g:\R \to \R^2$ be defined by $g(x,y) = (x, \sin(x))$.  
		\begin{solution}
			\begin{hint}
				\(\begin{bmatrix} 
				3a^2& 3b^2\\
				3a^2\cos(a^3+b^3)& 3b^2\cos(a^3+b^3)
				\end{bmatrix}\)
			\end{hint}
		Use the chain rule to find the
		Jacobian of $(g \circ f)$ at the point $(a,b)$.
		
		\begin{matrix-answer}
			correctMatrix = [['3a^2','3b^2'],['3a^2cos(a^3+b^3)','3b^2cos(a^3+b^3)']]
		\end{matrix-answer}
		\end{solution}
	\end{question}	
	
\end{document}
